---
type: problem
answers:
	- f'(x)g(x) + f(x)g'(x)

---

@statement
$\displaystyle{\frac{df(x)g(x)}{dx}}=$ 

@hint
Can\'t distribute? $$ab-cd$$ $$=ab-ad+ad-cd$$ $$=a(b-d)+d(a-c).$$ Yes you can.

@hint
What is $$\lim_{\delta x \to 0} \frac{f(x+\delta x)-f(x)}{\delta x}=??$$

@solution
1.  Set up the limit:

$$\lim_{\delta x \to 0} \frac{f(x+\delta x)g(x+\delta x) -f(x)g(x)}{\delta x}$$

  

2.  Apply the factorization rule (see Hint 1):

$$\lim_{\delta x \to 0} \frac{f(x+\delta x)g(x+\delta x)-f(x+\delta x)g(x)+f(x+\delta x)g(x) -f(x)g(x)}{\delta x}$$

  

3.  Separate:

$$\lim_{\delta x \to 0} \frac{f(x+\delta x)g(x+\delta x)-f(x+\delta x)g(x)}{\delta x}+ \lim_{\delta x \to 0}\frac{f(x+\delta x)g(x) -f(x)g(x)}{\delta x}$$

  

4.  Factor:

$$\lim_{\delta x \to 0}f(x+\delta x)\cdot\lim_{\delta x \to 0} \frac{g(x+\delta x)-g(x)}{\delta x}+ g(x)\lim_{\delta x \to 0}\frac{f(x+\delta x) -f(x)}{\delta x}$$

  

5.  These are just differentiations of $f(x)$ and $g(x)$! So, we can

substitute their differentiations:

  

$$\lim_{\delta x \to 0}f(x+\delta x)\cdot g'(x)+ g(x)f'(x)$$

  

6.  Finally, we approximate: $$\delta x \rightarrow 0$$

$$\frac{df(x)g(x)}{dx}=\boxed{ f(x)g'(x)+ g(x)f'(x)}$$

<!--stackedit_data:
eyJoaXN0b3J5IjpbMTQ4MTA5OTE3NSwtNzgxMDUxMDk3XX0=
-->