---
type: problem
answers:
	- 5

---

@statement
$\displaystyle{\frac{d\frac{f(x)}{g(x)}}{dx}}=$

@hint
Remember the distribution rule from the previous problem?

@hint 
Make two huge fractions, simplify, and add them.

@solution
1.  Set up the limit:

$$\lim_{\delta x \to 0} \frac{\frac{f(x+\delta x)}{g(x+\delta x)} -\frac{f(x)}{g(x)}}{\delta x}$$

  

2.  Apply the factorization rule (see Hint 1 from previous problem):

$$\lim_{\delta x \to 0} \frac{\frac{f(x+\delta x)}{g(x+\delta x)} -\frac{f(x+\delta x)}{g(x)}+\frac{f(x+\delta x)}{g(x)} -\frac{f(x)}{g(x)}}{\delta x}$$

  

3.  Separate:

$$\lim_{\delta x \to 0} \frac{\frac{f(x+\delta x)}{g(x+\delta x)} -\frac{f(x+\delta x)}{g(x)}}{\delta x}+\frac{\frac{f(x+\delta x)}{g(x)} -\frac{f(x)}{g(x)}}{\delta x}$$

  

4.  Combine:

$$\lim_{\delta x \to 0}\frac{f(x+\delta x)}{g(x)g(x+\delta x)}\cdot\frac{g(x) -g(x+\delta x)}{\delta x}+\frac{1}{g(x)}\cdot\frac{f(x+\delta x)-f(x)}{\delta x}$$

  

5.  These are just differentiations of $f(x)$ and $g(x)$! So, we can

substitute their differentiations:

  

$$\lim_{\delta x \to 0}\frac{f(x+\delta x)}{g(x)g(x+\delta x)}(-g'(x))+\frac{1}{g(x)}f'(x)$$

  

6.  Now, we approximate: $$\delta x \rightarrow 0$$

$$\frac{f(x)}{g(x)g(x)}g'(x)+\frac{f'(x)}{g(x)}$$

$$= \boxed{\frac{f'(x)g(x)-g'(x)f(x)}{(g(x))^2}}$$

<!--stackedit_data:
eyJoaXN0b3J5IjpbLTg2MzgzMjkzOF19
-->