---
type: lesson
title: Introduction
index: 0
description: Learn how to accurately approximate asymptotes of functions.
category: algebra
---

Limits are the basis for almost everything in calculus. By the time you get to derivatives, you'll be doing limits and
you won't even know it. To become familiar with what a limit is, let's consider the function

$$
f(x) = \frac{x^2-1}{x-1}.
$$
What is the value of this function at $x=1$?

$\frac{0}{0}$ is indeterminate, so the function $f(x)$ would be indeterminate at $x=1$. However, the function is defined
at $x=0.9$ and $x=1.1$:

$$
f(0.9) = 1.9
$$

$$
f(1.1) = 2.1
$$

In fact, the function is defined for any $1\pm \delta,$ where $\delta \neq 0.$

In this lesson, we'll be considering the case where $\delta$ is very close, but not equal to $0.$

<iframe src="https://www.desmos.com/calculator/ti0fuxp3s6?embed" class="graph" style="border: 1px solid #ccc;" id="graph1" frameborder="0"></iframe>

Try dragging the black point to $x=1$ in the above graph, and you will notice that the point disappears.

However, notice that it "looks like"

$$
f(1)=2.
$$

So, we can say that

$$
\lim_{x\to 1} f(x) = 2.
$$

The English for this is "As $x$ approaches 1, $f(x)$ approaches $2$."

Another possible interpretation is "The limit of $f(x)$ as $x$ approaches 1 is $2$."

This does not mean that $f(1)=2$ , but rather that if $x$ is very close to $1$, then is $f(x)$ very close to $2$.

Notice that the graphed function is linear. What linear function does it look like?

The function covers _almost all_ points covered by the function $x+1$.

We can confirm this by performing the following operation:

$$
\frac{x^2-1}{x-1} = \frac{(x-1)(x+1)}{x-1} = x+1
$$

> **Important!** This kind of math is only allowed in limits. Notice how we divided the top and bottom of the fraction by $x-1$, a non-constant â€“ we only did this knowing that $x$ is very close to, but not equal to 1.

Now try this:

$$
\lim_{x\to 2} \frac{x^2-5x+6}{x-2}.
$$

As we said before, it is okay to divide by non-constants in limits. So, we can say

$$
\lim_{x\to 2} \frac{x^2-5x+6}{x-2} = \lim_{x\to 2} x-3.
$$

We can just plug in $x=2$ here to find

$$
\lim_{x\to 2} \frac{x^2-5x+6}{x-2} = -1.
$$
