---
type: problem
answers:
  - "done"
---

@statement
Show how the Pythagorean Theorem is a sub-case of the Law of Cosines. Type "done" in the answer box when you are done.

@hint
What terms do we need to remove to get the Pythagorean Theorem?

@solution
If we let $\angle C = 90$, then $\cos \angle C = 0$, meaning $-2ab \cos \angle C = 0$. Our equation then becomes: $$c^2 = a^2 + b^2$$
which is the Pythagorean Theorem. We see that it is true when angle C is 90 degrees, or a right angle!.This is of course not a proof for the Pythagorean Theorem, as we used the theorem to prove the Law of Cosines in the first place. It's just a neat side result!
<!--stackedit_data:
eyJoaXN0b3J5IjpbNjA3NTg3MzAyLDEyOTc4MTI1LC00NzUzMT
Q0MDFdfQ==
-->