---
type: problem
answers:
  - "m^3n^3"
  - "m^3 n^3"
  - "m^3\cdot n^3"
  - "n^3m^3"
  - "n^3 m^3"
  - "n^3\cdot m^3"

---

@statement
Expand and simplify $(pq)^3$.

@hint
Plug in values into the Power of a Product rule. 

@hint
You could also try rewriting the expression as repeated multiplication. 

@solution
By the Power of a Product rule, $(pq)^3=p^3q^3$. We can also write this as repeated multiplication. 
$$(pq)^3=(pq)(pq)(pq)=(ppp)(qqq)=p^3q^3$$
<!--stackedit_data:
eyJoaXN0b3J5IjpbLTEwNjE2MDU5ODhdfQ==
-->