---
type: problem
answers:
  - $\frac{p^tq^t}{r^ts^t}$

---

@statement
Expand and simplify $\left(\frac{pq}{rs}\right)^t$. 

@hint
Rewrite $\frac{pq}{rs}$ as the product of two fractions.

@hint
Use both the Power of a Product Rule and the Power of a Quotient Rule.

@solution
We write $\frac{pq}{rs}$ as $\frac pr \cdot \frac qs$. Then, we apply the Power of a Product and Power of a Quotient Rules.
$$\left(\frac{pq}{rs}\right)^t
= \left(\frac pr \cdot \frac qs\right)^t
= \left(\frac pr\right)^t\left(\frac qs\right)^t
= \left(\frac{p^t}{r^t}\right)\left(\frac{q^t}{s^t}\right)
=\frac{p^tq^t}{r^ts^t}$$
Note that there are many different ways to solve this problem, and they all lead to the same solution. 
<!--stackedit_data:
eyJoaXN0b3J5IjpbLTMyODk5NTg3NCw4MTg3MTk5NTNdfQ==
-->